src/BinEncoders/Env/Lib2/DomainNameOpt.v
@@ -10,6 +10,7 @@ Require Import
         Fiat.Examples.DnsServer.Packet
         Fiat.BinEncoders.Env.Common.Specs
         Fiat.BinEncoders.Env.Lib2.FixStringOpt
+        Fiat.BinEncoders.Env.Lib2.NatOpt
         Fiat.BinEncoders.Env.Lib2.WordOpt
         Fiat.BinEncoders.Env.Lib2.AsciiOpt.
 
@@ -19,11 +20,24 @@ Section DomainName.
   Context {cache_inv : CacheDecode -> Prop}.
   Context {cacheAddNat : CacheAdd cache nat}.
   Context {transformer : Transformer B}.
-  Context {transformerUnit : TransformerUnitOpt transformer bool}.
+  Context {transformerUnit : QueueTransformerOpt transformer bool}.
 
   (* The terminal character for domain names is the byte of all zeros. *)
   Definition terminal_char : ascii := zero.
-  Definition pointerT := word 6.
+  Definition pointerT := (word 8 * word 8)%type.
+
+  Lemma terminal_char_eq :
+    forall x0, terminal_char = ascii_of_N (wordToN x0)
+               -> x0 = wzero 8.
+  Proof.
+    intros.
+    unfold terminal_char, zero in H.
+    shatter_word x0.
+    simpl in H.
+    repeat (find_if_inside; simpl in H);
+      try discriminate.
+    reflexivity.
+  Qed.
 
   Context {cacheAdd : CacheAdd cache (string * pointerT)}.
   Context {cacheGet : CacheGet cache string pointerT}.
@@ -55,7 +69,9 @@ Section DomainName.
     (Ifopt (getE env domain) as position Then
         b <- {b : bool | True};
           If b Then (* Nondeterministically pick whether to use a cached value. *)
-             (encode_word_Spec position env)
+             (`(ptr1b, env') <- encode_word_Spec (fst position) env;
+              `(ptr2b, env') <- encode_word_Spec (snd position) env';
+              ret (transform ptr1b ptr2b, env'))
              Else (`(label, domain') <- { labeldomain' |
                                           domain = (fst labeldomain') ++ (snd labeldomain')
                                           /\ ValidLabel (fst labeldomain')
@@ -63,10 +79,10 @@ Section DomainName.
                                                  domain = label' ++ post'
                                                  -> ValidLabel label'
                                                  -> String.length label' <= String.length (fst labeldomain'))}%string%nat;
-                     `(lenb, env') <- encode_word_Spec (natToWord 8 (String.length label)) env;
+                     `(lenb, env') <- encode_nat_Spec 8 (String.length label) env;
                      `(labelb, env') <- encode_string_Spec label env';
                      `(domainb, env') <- encode_DomainName_Spec domain' env';
-                     ret (transform (transform lenb labelb) domainb, addE env (domain, peekE env)))
+                     ret (transform (transform lenb labelb) domainb, addE env' (domain, peekE env)))
              Else
              (`(label, domain') <- { labeldomain' |
                                           domain = (fst labeldomain') ++ (snd labeldomain')
@@ -75,27 +91,26 @@ Section DomainName.
                                                  domain = label' ++ post'
                                                  -> ValidLabel label'
                                                  -> String.length label' <= String.length (fst labeldomain'))}%string%nat;
-                     `(lenb, env') <- encode_word_Spec (natToWord 8 (String.length label)) env;
+                     `(lenb, env') <- encode_nat_Spec 8 (String.length label) env;
                      `(labelb, env') <- encode_string_Spec label env';
                      `(domainb, env') <- encode_DomainName_Spec domain' env';
-                     ret (transform (transform lenb labelb) domainb, addE env (domain, peekE env))))) domain env.
+                     ret (transform (transform lenb labelb) domainb, addE env' (domain, peekE env))))) domain env.
 
   (* Decode now uses a measure on the length of B *)
 
   Lemma lt_B_trans :
     forall b
            (b1 : {b' : B | le_B b' b})
-           (b2 : {b' : B | lt_B b' (` b1)})
-           (b3 : {b' : B | lt_B b' (` b2)}),
+           (b3 : {b' : B | lt_B b' (` b1)}),
       lt_B (` b3) b.
   Proof.
-    intros; destruct b1; destruct b2; destruct b3; simpl in *.
+    intros; destruct b1; destruct b3; simpl in *.
     unfold le_B, lt_B in *; omega.
   Qed.
 
   Lemma n_eq_0_lt :
     forall n,
-      n <> wzero 6
+      n <> wzero 8
       -> (0 < wordToNat n)%nat.
   Proof.
     induction n; unfold wzero; simpl.
@@ -108,175 +123,494 @@ Section DomainName.
       omega.
   Qed.
 
+  Lemma append_assoc :
+    forall s1 s2 s3,
+      (s1 ++ s2 ++ s3 = (s1 ++ s2) ++ s3)%string.
+  Proof.
+    induction s1; simpl; auto.
+    intros; rewrite IHs1; reflexivity.
+  Qed.
+
+  Lemma length_append :
+    forall s1 s2,
+      String.length (s1 ++ s2) = String.length s1 + String.length s2.
+  Proof.
+    induction s1; simpl; eauto.
+  Qed.
+
+  Lemma ValidDomainName_app
+    : forall label subdomain,
+      ValidLabel label ->
+      ValidDomainName (label ++ subdomain)
+      -> ValidDomainName subdomain.
+  Proof.
+    unfold ValidDomainName; intros.
+    eapply H0; try eassumption.
+    rewrite H1.
+    rewrite append_assoc.
+    reflexivity.
+  Qed.
+
+  Lemma chomp_label_length
+    : forall n label subdomain,
+      (String.length (label ++ subdomain) <= S n)%nat
+      -> ValidLabel label
+      -> (String.length subdomain <= n)%nat.
+  Proof.
+    destruct label.
+    - unfold ValidLabel; simpl; intros; omega.
+    - intro subdomain; rewrite length_append; simpl.
+      omega.
+  Qed.
+
   Definition decode_DomainName (b : B) (env : CacheDecode):
     option (DomainName * B * CacheDecode).
     refine (Fix well_founded_lt_b
            (fun _ => CacheDecode -> option (DomainName * B * CacheDecode))
       (fun b rec cd =>
-         `(labelheader, b1, env') <- Decode_w_Measure_le (decode_word (sz := 2)) b env _;
-           If (weq labelheader WO~1~1) (* It's a pointer! *)
-           Then (`(ps, b2, env') <- Decode_w_Measure_le (decode_word (sz := 6)) (proj1_sig b1) env' _;
-               match getD cd ps with
+         `(labelheader, b1, env') <- Decode_w_Measure_le (decode_word (sz := 8)) b cd _;
+           If (wlt_dec (natToWord 8 191) labelheader) (* It's a pointer! *)
+           Then (`(ps, b2, env') <- Decode_w_Measure_le (decode_word (sz := 8)) (proj1_sig b1) env' decode_word_le;
+               match getD cd (labelheader, ps) with
                  | Some EmptyString => None (* bogus *)
                  | Some domain => Some (domain, proj1_sig b2, env')
                  | None => None (* bogus *)
                  end)
-           Else (If (weq labelheader WO~0~0) Then (* It's a length octet *)
-         (`(labellength, b2, env') <- Decode_w_Measure_lt (decode_word (sz := 6)) (proj1_sig b1) env' _;
-            match (weq labellength (wzero 6)) with (* It's the terminal character. *)
-              | left _ => Some (EmptyString, proj1_sig b2, env')
-              | right _ =>
-             (`(label, b3, env') <- Decode_w_Measure_lt (decode_string (wordToNat labellength))
-               (proj1_sig b2) env' _;
-              `(domain, b4, e3) <- rec (proj1_sig b3) _ env';
-              Some (label ++ domain, b4, addD env' (label ++ domain, peekD env))) end)
+           Else (If (wlt_dec labelheader (natToWord 8 64)) Then (* It's a length octet *)
+         (match (weq labelheader (wzero 8)) with (* It's the terminal character. *)
+              | left _ => Some (EmptyString, proj1_sig b1, env')
+              | right n =>
+             (`(label, b3, env') <- Decode_w_Measure_lt (decode_string (wordToNat labelheader))
+               (proj1_sig b1) env' (decode_string_lt _ (n_eq_0_lt _ n));
+              `(domain, b4, e3) <- rec (proj1_sig b3) (lt_B_trans _ _ _) env';
+              Some (label ++ domain, b4, addD e3 (label ++ domain, peekD cd))) end)
          Else None))%string b env);
-      try solve [intros; unfold decode_word; eapply decode_word_lt; eauto];
-      try solve [intros; eapply decode_word_le; eauto].
-    intros; eapply decode_string_lt; try eapply H.
-    apply n_eq_0_lt; eauto.
-    apply lt_B_trans.
+    try exact decode_word_le;
+      try exact decode_word_lt.
   Defined.
 
+  Lemma decode_body_monotone
+    : forall (x : B)
+     (f g : forall y : B, lt_B y x -> CacheDecode -> option (DomainName * B * CacheDecode)),
+   (forall (y : B) (p : lt_B y x), f y p = g y p) ->
+   (fun cd : CacheDecode =>
+    `(labelheader, b1, env') <- Decode_w_Measure_le decode_word x cd decode_word_le;
+    If wlt_dec WO~1~0~1~1~1~1~1~1 labelheader
+    Then `(ps, b2, env'0) <- Decode_w_Measure_le decode_word (` b1) env' decode_word_le;
+         match getD cd (labelheader, ps) with
+         | Some ""%string => None
+         | Some (String _ _ as domain) => Some (domain, ` b2, env'0)
+         | None => None
+         end
+    Else (If wlt_dec labelheader WO~0~1~0~0~0~0~0~0
+          Then match weq labelheader (wzero 8) with
+               | in_left => Some (""%string, ` b1, env')
+               | right n =>
+                   `(label, b3, env'0) <- Decode_w_Measure_lt
+                                            (decode_string (wordToNat labelheader)) 
+                                            (` b1) env'
+                                            (decode_string_lt 
+                                               (wordToNat labelheader)
+                                               (n_eq_0_lt labelheader n));
+                   `(domain, b4, e3) <- f (` b3) (lt_B_trans x b1 b3) env'0;
+                   Some
+                     ((label ++ domain)%string, b4,
+                     addD e3 ((label ++ domain)%string, peekD cd))
+               end Else None)) =
+   (fun cd : CacheDecode =>
+    `(labelheader, b1, env') <- Decode_w_Measure_le decode_word x cd decode_word_le;
+    If wlt_dec WO~1~0~1~1~1~1~1~1 labelheader
+    Then `(ps, b2, env'0) <- Decode_w_Measure_le decode_word (` b1) env' decode_word_le;
+         match getD cd (labelheader, ps) with
+         | Some ""%string => None
+         | Some (String _ _ as domain) => Some (domain, ` b2, env'0)
+         | None => None
+         end
+    Else (If wlt_dec labelheader WO~0~1~0~0~0~0~0~0
+          Then match weq labelheader (wzero 8) with
+               | in_left => Some (""%string, ` b1, env')
+               | right n =>
+                   `(label, b3, env'0) <- Decode_w_Measure_lt
+                                            (decode_string (wordToNat labelheader)) 
+                                            (` b1) env'
+                                            (decode_string_lt 
+                                               (wordToNat labelheader)
+                                               (n_eq_0_lt labelheader n));
+                   `(domain, b4, e3) <- g (` b3) (lt_B_trans x b1 b3) env'0;
+                   Some
+                     ((label ++ domain)%string, b4,
+                     addD e3 ((label ++ domain)%string, peekD cd))
+               end Else None)).
+  Proof.
+    intros; apply functional_extensionality; intros.
+    repeat (f_equal; apply functional_extensionality; intros).
+    destruct (wlt_dec WO~1~0~1~1~1~1~1~1 x1); simpl.
+    repeat (f_equal; apply functional_extensionality; intros).
+    destruct (wlt_dec x1 WO~0~1~0~0~0~0~0~0); simpl.
+    destruct (weq x1 (wzero 8)).
+    reflexivity.
+    repeat (f_equal; apply functional_extensionality; intros);
+      rewrite H; reflexivity.
+    reflexivity.
+  Qed.
+  
+  Lemma encode_body_monotone
+    : forall rec rec' : funType [DomainName; CacheEncode] (B * CacheEncode),
+   refineFun rec rec' ->
+   refineFun (fDom := [DomainName; CacheEncode])
+     (fun (domain : DomainName) (env0 : CacheEncode) =>
+      If string_dec domain "" Then encode_ascii_Spec terminal_char env0
+      Else (Ifopt getE env0 domain as position
+            Then b <- {_ : bool | True};
+                 If b
+                 Then `(ptr1b, env') <- encode_word_Spec (fst position) env0;
+                      `(ptr2b, env'0) <- encode_word_Spec (snd position) env';
+                      ret (transform ptr1b ptr2b, env'0)
+                 Else (`(label, domain') <- {labeldomain' :
+                                            string * string |
+                                            domain =
+                                            (fst labeldomain' ++ snd labeldomain')%string /\
+                                            ValidLabel (fst labeldomain') /\
+                                            (forall label' post' : string,
+                                             domain = (label' ++ post')%string ->
+                                             ValidLabel label' ->
+                                             (String.length label' <=
+                                              String.length (fst labeldomain'))%nat)};
+                       `(lenb, env') <- encode_nat_Spec 8 (String.length label) env0;
+                       `(labelb, env'0) <- encode_string_Spec label env';
+                       `(domainb, env'1) <- rec domain' env'0;
+                       ret
+                         (transform (transform lenb labelb) domainb,
+                         addE env'1 (domain, peekE env0)))
+            Else (`(label, domain') <- {labeldomain' :
+                                       string * string |
+                                       domain = (fst labeldomain' ++ snd labeldomain')%string /\
+                                       ValidLabel (fst labeldomain') /\
+                                       (forall label' post' : string,
+                                        domain = (label' ++ post')%string ->
+                                        ValidLabel label' ->
+                                        (String.length label' <=
+                                         String.length (fst labeldomain'))%nat)};
+                  `(lenb, env') <- encode_nat_Spec 8 (String.length label) env0;
+                  `(labelb, env'0) <- encode_string_Spec label env';
+                  `(domainb, env'1) <- rec domain' env'0;
+                  ret
+                    (transform (transform lenb labelb) domainb,
+                    addE env'1 (domain, peekE env0)))))
+     (fun (domain : DomainName) (env0 : CacheEncode) =>
+      If string_dec domain "" Then encode_ascii_Spec terminal_char env0
+      Else (Ifopt getE env0 domain as position
+            Then b <- {_ : bool | True};
+                 If b
+                 Then `(ptr1b, env') <- encode_word_Spec (fst position) env0;
+                      `(ptr2b, env'0) <- encode_word_Spec (snd position) env';
+                      ret (transform ptr1b ptr2b, env'0)
+                 Else (`(label, domain') <- {labeldomain' :
+                                            string * string |
+                                            domain =
+                                            (fst labeldomain' ++ snd labeldomain')%string /\
+                                            ValidLabel (fst labeldomain') /\
+                                            (forall label' post' : string,
+                                             domain = (label' ++ post')%string ->
+                                             ValidLabel label' ->
+                                             (String.length label' <=
+                                              String.length (fst labeldomain'))%nat)};
+                       `(lenb, env') <- encode_nat_Spec 8 (String.length label) env0;
+                       `(labelb, env'0) <- encode_string_Spec label env';
+                       `(domainb, env'1) <- rec' domain' env'0;
+                       ret
+                         (transform (transform lenb labelb) domainb,
+                         addE env'1 (domain, peekE env0)))
+            Else (`(label, domain') <- {labeldomain' :
+                                       string * string |
+                                       domain = (fst labeldomain' ++ snd labeldomain')%string /\
+                                       ValidLabel (fst labeldomain') /\
+                                       (forall label' post' : string,
+                                        domain = (label' ++ post')%string ->
+                                        ValidLabel label' ->
+                                        (String.length label' <=
+                                         String.length (fst labeldomain'))%nat)};
+                  `(lenb, env') <- encode_nat_Spec 8 (String.length label) env0;
+                  `(labelb, env'0) <- encode_string_Spec label env';
+                  `(domainb, env'1) <- rec' domain' env'0;
+                  ret
+                    (transform (transform lenb labelb) domainb,
+                    addE env'1 (domain, peekE env0))))).
+  Proof.
+    simpl; intros; unfold Bind2.
+    apply General.refine_if; intros; rewrite H0; simpl.
+    reflexivity.
+    apply SetoidMorphisms.refine_If_Opt_Then_Else_Proper.
+    * intro; f_equiv; intro.
+      apply General.refine_if; intros H5; rewrite H5; simpl;
+        unfold Bind2; f_equiv; intro.
+      setoid_rewrite H; reflexivity.
+    * f_equiv; intro.
+      unfold Bind2; f_equiv; intro.
+      setoid_rewrite H; reflexivity.
+  Qed.
+
   (* Commenting out until I can patch up proof. *)
-  (*Theorem DomainName_decode_correct :
+  Theorem DomainName_decode_correct
+          {P : CacheDecode -> Prop}
+          (P_OK : cache_inv_Property P (fun P => forall (b : nat) cd, P cd -> P (addD cd b)))
+          (Get_P_OK
+           : cache_inv_Property P
+                                (fun P => forall ce l p1 p2,
+                                     (@getE _ DomainName _ _ ce l = Some (p1, p2)
+                                      -> wlt (natToWord 8 191) p1)))
+    :
     encode_decode_correct_f
       cache transformer
-      (fun domain => ValidDomainName domain /\ (String.length domain > 0)%nat)
-      encode_DomainName_Spec decode_DomainName cache_inv.
+      (fun domain => ValidDomainName domain)
+      (fun _ _ => True)
+      encode_DomainName_Spec decode_DomainName P.
   Proof.
     unfold encode_decode_correct_f; split.
-    { intros env xenv xenv' l l' ext Eeq Ppredh Penc;
-      subst.
+    { intros env xenv xenv' l l' ext Eeq Valid_data
+             Ppred_rest Penc.
       unfold decode_DomainName in *; simpl in *.
       unfold encode_DomainName_Spec in Penc.
+      simpl in *.
       generalize dependent l';
         generalize dependent env;
         generalize dependent xenv;
-        generalize ext; generalize dependent xenv';
-          induction l; intros; simpl in *.
-      { unfold Bind2 in *; computes_to_inv; subst.
-        destruct v; destruct v0.
-        injections.
-        destruct (proj1 X_decode_pf _ _ _ _ _ (transform b0 ext0) Eeq I Penc) as [? [? ?]]; subst.
-        rewrite <- transform_assoc.
-        rewrite Coq.Init.Wf.Fix_eq; simpl.
-        let H' := fresh in
-        destruct (Decode_w_Measure_le_eq _ _ _ X_decode_le H) as [? H'];
-          rewrite H'; simpl; clear H'.
-          destruct (proj1 A_decode_pf _ _ _ _ _ ext0 H0 A_predicate_halt Penc') as [? [? ?]]; subst.
-          let H' := fresh in
-          destruct (Decode_w_Measure_lt_eq _ _ _ A_decode_lt H1) as [? H'];
-            rewrite H'; simpl; clear H'.
-          destruct (A_halt_dec A_halt); simpl; eexists; eauto.
-          congruence.
-          intros.
-          apply functional_extensionality; intros.
-          repeat (f_equal; repeat (apply functional_extensionality; intros)).
+        generalize ext; generalize dependent xenv'.
+      generalize (Le.le_refl (String.length l)) as le_n.
+      remember (String.length l) as n.
+      rewrite Heqn at 1.
+      clear Heqn; generalize dependent l.
+      induction n; intros; simpl in *.
+      destruct l; simpl in *; try omega.
+      { apply (unroll_LeastFixedPoint (fDom := [DomainName; CacheEncode]) (fCod := (B * CacheEncode))) in Penc; auto using encode_body_monotone; simpl in Penc.
+         destruct (proj1 (Ascii_decode_correct P_OK)
+                        _ _ _ _ _ ext0 Eeq I I Penc) as [? [? ?] ].
+        apply DecodeBindOpt2_inv in H0;
+          destruct H0 as [? [? [? [? ?] ] ] ]; injections; subst.
+        eexists; split.
+        + unfold encode_ascii_Spec, encode_word_Spec in Penc;
+          computes_to_inv; subst; simpl in *; injections.
+          rewrite Init.Wf.Fix_eq; auto using decode_body_monotone; simpl.
+          match goal with
+            |- context [Decode_w_Measure_le ?x ?y ?z ?m] =>
+            destruct (Decode_w_Measure_le_eq x y z m H0) as [? H2];
+              rewrite H2
+          end.
+          apply terminal_char_eq in H5; rewrite H5.
+          reflexivity.
+        + auto.
       }
-      destruct (getE env (a :: l)) eqn: ?.
-      rewrite Coq.Init.Wf.Fix_eq; simpl.
-      computes_to_inv.
-      destruct v; simpl in Penc'.
-      { (* Case where the encoder decided to use compression. *)
-        destruct (P_predicate_dec p); simpl in Penc';
-        unfold Bind2 in Penc'; computes_to_inv; injections;
-        subst; destruct v; destruct v0.
-        - destruct (proj1 X_decode_pf _ _ _ _ _ (transform b0 ext0) Eeq I Penc') as [? [? ?]]; subst.
-          rewrite <- transform_assoc; simpl;
-            let H' := fresh in
-            destruct (Decode_w_Measure_le_eq _ _ _ X_decode_le H) as [? H'];
-              rewrite H'; simpl; clear H'.
-          destruct (proj1 P_decode_pf _ _ _ _ _ ext0 H0 p0 Penc'') as [? [? ?]];
-           let H' := fresh in
-            destruct (Decode_w_Measure_le_eq _ _ _ P_decode_le H1) as [? H'];
-              rewrite H'; simpl; clear H'.
-          eapply get_correct in Heqo; eauto; rewrite Heqo.
-          eauto.
-        - destruct v1.
-          destruct (proj1 X_decode_pf _ _ _ _ _ (transform b0 (transform b1 ext0))
-                          Eeq I Penc') as [? [? ?]]; subst.
-          rewrite <- !transform_assoc; simpl.
-          let H' := fresh in
-          destruct (Decode_w_Measure_le_eq _ _ _ X_decode_le H) as [? H'];
-            rewrite H'; simpl; clear H'.
-          destruct (proj1 A_decode_pf _ _ _ _ _ (transform b1 ext0) H0 (proj1 (Ppredh _ (or_introl _ eq_refl))) Penc'') as [? [? ?]]; subst.
-          let H' := fresh in
-          destruct (Decode_w_Measure_lt_eq _ _ _ A_decode_lt H1) as [? H'];
-            rewrite H'; simpl; clear H'.
-          destruct (A_halt_dec a); simpl.
-          elimtype False; apply (proj2 (Ppredh _ (or_introl _ eq_refl)));
-            eauto.
-          eapply (fun H => IHl H _ ext0) in Penc'''; intros.
-          destruct_ex; intuition.
-          rewrite H4; simpl.
-          eexists; intuition eauto.
-          erewrite peek_correct.
-          eapply add_correct.
-          eauto.
-          eauto.
-          eapply Ppredh; eauto.
-          eauto.
+      { apply (unroll_LeastFixedPoint (fDom := [DomainName; CacheEncode]) (fCod := (B * CacheEncode))) in Penc; auto using encode_body_monotone.
+        { destruct (string_dec l ""); simpl in Penc.
+          (* Base case for domain name. *)
+          - destruct (proj1 (Ascii_decode_correct P_OK)
+                            _ _ _ _ _ ext0 Eeq I I Penc) as [? [? ?] ].
+            apply DecodeBindOpt2_inv in H0;
+              destruct H0 as [? [? [? [? ?] ] ] ]; injections; subst.
+            eexists; split.
+            + unfold encode_ascii_Spec, encode_word_Spec in Penc;
+                computes_to_inv; subst; simpl in *; injections.
+              rewrite Init.Wf.Fix_eq; auto using decode_body_monotone; simpl.
+              match goal with
+                |- context [Decode_w_Measure_le ?x ?y ?z ?m] =>
+                destruct (Decode_w_Measure_le_eq x y z m H0) as [? H2];
+                  rewrite H2
+              end.
+              apply terminal_char_eq in H5; rewrite H5.
+              reflexivity.
+            + assumption.
+          - destruct (@getE _ DomainName _ _ env l) as [ [ptr1 ptr2] | ] eqn:GetPtr;
+              simpl in Penc; computes_to_inv.
+            { (* pointer found *)
+              destruct v; simpl in Penc'; unfold Bind2 in Penc'; computes_to_inv.
+              - (* Encoder chose to use compression. *)
+                destruct v as [b xenv'']; destruct v0 as [b' xenv'''];
+                  simpl in *; injections.
+                unfold encode_word_Spec in Penc', Penc'';
+                  computes_to_inv; subst; simpl in *; injections.
+                eexists; split.
+                rewrite Init.Wf.Fix_eq; simpl.
+                + match goal with
+                    |- context [Decode_w_Measure_le ?x ?y ?z ?m] =>
+                    pose proof (Decode_w_Measure_le_eq x y z m)
+                  end.
+                  simpl in H0;
+                    unfold decode_word at 1 in H0;
+                    rewrite <- transform_assoc,
+                    <- transformer_dequeue_word_eq_decode_word',
+                    transformer_dequeue_encode_word' in H0;
+                    simpl in H0;
+                    destruct (H0 _ _ _ (eq_refl _)) as [? H']; clear H0.
+                  rewrite <- transform_assoc, H'; simpl.
+                  destruct (wlt_dec WO~1~0~1~1~1~1~1~1 ptr1); simpl.
+                  * match goal with
+                      |- context [Decode_w_Measure_le ?x ?y ?z ?m] =>
+                      pose proof (Decode_w_Measure_le_eq x y z m)
+                    end.
+                    simpl in H0;
+                      unfold decode_word at 1 in H0;
+                      rewrite <- transformer_dequeue_word_eq_decode_word',
+                      transformer_dequeue_encode_word' in H0;
+                      simpl in H0;
+                      destruct (H0 _ _ _ (eq_refl _)) as [? H'']; clear H0;
+                        rewrite H''; clear H''; simpl.
+                    eapply get_correct in GetPtr; eauto;
+                      unfold DomainName, pointerT in *; rewrite GetPtr.
+                    destruct l; try congruence.
+                    reflexivity.
+                  * apply Get_P_OK in GetPtr; contradiction.
+                + intros; apply functional_extensionality; intros.
+                  repeat (f_equal; apply functional_extensionality; intros).
+                  destruct (wlt_dec WO~1~0~1~1~1~1~1~1 x1); simpl.
+                  repeat (f_equal; apply functional_extensionality; intros).
+                  destruct (wlt_dec x1 WO~0~1~0~0~0~0~0~0); simpl.
+                  destruct (weq x1 (wzero 8)).
+                  reflexivity.
+                  repeat (f_equal; apply functional_extensionality; intros).
+                  rewrite H0; reflexivity.
+                  reflexivity.
+                + repeat apply add_correct; eauto.
+              - (* Encoder chose not to compress *)
+                destruct Penc' as [l_eq [label1_OK label1_OK'] ].
+                destruct v as [label1 label2]; destruct v0 as [b' xenv'''];
+                  destruct v1 as [b'' xenv'''']; destruct v2 as [b3 xenv5];
+                    simpl in *; injections.
+                destruct (fun H => proj1 (Nat_decode_correct (P := fun _ => True) 8 (fun _ _ _ => I)) _ _ _ _ _ (transform b'' (transform b3 ext0)) Eeq H I Penc'') as [xenv4 [? xenv_eqv] ].
+                pose proof (Valid_data ""%string label1 label2 (eq_refl _) label1_OK).
+                simpl; omega.
+                destruct (fun H => proj1 (String_decode_correct (P := fun _ => True) (fun _ _ _ => I) (String.length label1)) _ _ _ _ _ (transform b3 ext0) xenv_eqv H I Penc''') as [xenv6 [? xenv6_eqv] ]; eauto.
+                eapply IHn in Penc''''.
+                destruct Penc'''' as [xenv7 [? ?] ].
+                eexists; split.
+                rewrite Init.Wf.Fix_eq; auto using decode_body_monotone; simpl.
+                + match goal with
+                    |- context [Decode_w_Measure_le ?x ?y ?z ?m] =>
+                    pose proof (Decode_w_Measure_le_eq x y z m)
+                  end.
+                  simpl in H4;
+                    unfold decode_word at 1 in H4.
+                  rewrite <- !transform_assoc in H4.
+                  unfold decode_nat in H0.
+                  apply DecodeBindOpt2_inv in H0;
+                    destruct H0 as [? [? [? [? ?] ] ] ]; injections; subst.
+                  unfold decode_word in H0.
+                  destruct (decode_word' 8 (transform b' (transform b'' (transform b3 ext0)))); simpl in H0; try discriminate; injections.
+                  simpl in H4.
+                  destruct (H4 _ _ _ (eq_refl _)).
+                  rewrite <- !transform_assoc, H0; simpl; clear H0.
+                  pose proof (Valid_data ""%string label1 label2 (eq_refl _) label1_OK) as w';
+                    rewrite H8 in w'.
+                  destruct (wlt_dec WO~1~0~1~1~1~1~1~1 x); simpl;
+                    try (apply WordFacts.wordToNat_lt in w; simpl in w; omega).
+                  destruct (wlt_dec x WO~0~1~0~0~0~0~0~0); simpl.
+                  * destruct (weq x (wzero 8)).
+                    subst; simpl in H8.
+                    destruct label1; simpl in H8; try discriminate.
+                    unfold ValidLabel in label1_OK; simpl in label1_OK; omega.
+                    match goal with
+                      |- context [Decode_w_Measure_lt ?x ?y ?z ?m] =>
+                      pose proof (Decode_w_Measure_lt_eq x y z m)
+                    end.
+                    simpl in H0; rewrite H8 in H1; rewrite H1 in H0.
+                    destruct (H0 _ _ _ (eq_refl _)).
+                    rewrite H5; simpl; rewrite H2; reflexivity.
+                  * destruct n2.
+                    rewrite <- natToWord_wordToNat;
+                      rewrite <- (natToWord_wordToNat x).
+                    apply WordFacts.natToWord_wlt.
+                    simpl.
+                    apply Nomega.Nlt_in.
+                    rewrite Nnat.Nat2N.id; etransitivity; eauto.
+                    simpl. unfold BinPos.Pos.to_nat; simpl.
+                    omega.
+                    apply Nomega.Nlt_in.
+                    simpl. unfold BinPos.Pos.to_nat; simpl.
+                    omega.
+                    simpl; omega.
+                + erewrite peek_correct.
+                  apply add_correct; eauto.
+                  eauto.
+                + eauto using ValidDomainName_app.
+                + eauto using chomp_label_length.
+                + eassumption.
+            }
+            { (* No pointer available *)
+              unfold Bind2 in Penc; computes_to_inv.
+              destruct Penc as [l_eq [label1_OK label1_OK'] ].
+              destruct v as [label1 label2]; destruct v0 as [b' xenv'''];
+                destruct v1 as [b'' xenv'''']; destruct v2 as [b3 xenv5];
+                  simpl in *; injections.
+              destruct (fun H => proj1 (Nat_decode_correct (P := fun _ => True) 8 (fun _ _ _ => I)) _ _ _ _ _ (transform b'' (transform b3 ext0)) Eeq H I Penc') as [xenv4 [? xenv_eqv] ].
+              pose proof (Valid_data ""%string label1 label2 (eq_refl _) label1_OK).
+              simpl; omega.
+              destruct (fun H => proj1 (String_decode_correct (P := fun _ => True) (fun _ _ _ => I) (String.length label1)) _ _ _ _ _ (transform b3 ext0) xenv_eqv H I Penc'') as [xenv6 [? xenv6_eqv] ]; eauto.
+              eapply IHn in Penc'''.
+              destruct Penc''' as [xenv7 [? ?] ].
+              eexists; split.
+              rewrite Init.Wf.Fix_eq; auto using decode_body_monotone; simpl.
+              + match goal with
+                  |- context [Decode_w_Measure_le ?x ?y ?z ?m] =>
+                  pose proof (Decode_w_Measure_le_eq x y z m)
+                end.
+                simpl in H4;
+                  unfold decode_word at 1 in H4.
+                rewrite <- !transform_assoc in H4.
+                unfold decode_nat in H0.
+                apply DecodeBindOpt2_inv in H0;
+                  destruct H0 as [? [? [? [? ?] ] ] ]; injections; subst.
+                unfold decode_word in H0.
+                destruct (decode_word' 8 (transform b' (transform b'' (transform b3 ext0)))); simpl in H0; try discriminate; injections.
+                simpl in H4.
+                destruct (H4 _ _ _ (eq_refl _)).
+                rewrite <- !transform_assoc, H0; simpl; clear H0.
+                pose proof (Valid_data ""%string label1 label2 (eq_refl _) label1_OK) as w';
+                  rewrite H8 in w'.
+                destruct (wlt_dec WO~1~0~1~1~1~1~1~1 x); simpl;
+                  try (apply WordFacts.wordToNat_lt in w; simpl in w; omega).
+                destruct (wlt_dec x WO~0~1~0~0~0~0~0~0); simpl.
+                * destruct (weq x (wzero 8)).
+                  subst; simpl in H8.
+                  destruct label1; simpl in H8; try discriminate.
+                  unfold ValidLabel in label1_OK; simpl in label1_OK; omega.
+                  match goal with
+                    |- context [Decode_w_Measure_lt ?x ?y ?z ?m] =>
+                    pose proof (Decode_w_Measure_lt_eq x y z m)
+                  end.
+                  simpl in H0; rewrite H8 in H1; rewrite H1 in H0.
+                  destruct (H0 _ _ _ (eq_refl _)).
+                  rewrite H5; simpl; rewrite H2; reflexivity.
+                * destruct n2.
+                  rewrite <- natToWord_wordToNat;
+                    rewrite <- (natToWord_wordToNat x).
+                  apply WordFacts.natToWord_wlt.
+                  simpl.
+                  apply Nomega.Nlt_in.
+                  rewrite Nnat.Nat2N.id; etransitivity; eauto.
+                  simpl. unfold BinPos.Pos.to_nat; simpl.
+                  omega.
+                  apply Nomega.Nlt_in.
+                  simpl. unfold BinPos.Pos.to_nat; simpl.
+                  omega.
+                  simpl; omega.
+              + erewrite peek_correct.
+                apply add_correct; eauto.
+                eauto.
+              + eauto using ValidDomainName_app.
+              + eauto using chomp_label_length.
+              + eassumption.
+            }
+        }
       }
-      {
-        unfold Bind2 in Penc'; computes_to_inv; injections;
-        subst; destruct v; destruct v0; destruct v1.
-        - destruct (proj1 X_decode_pf _ _ _ _ _ (transform b0 (transform b1 ext0)) Eeq I Penc') as [? [? ?]]; subst.
-          rewrite <- !transform_assoc; simpl.
-          let H' := fresh in
-          destruct (Decode_w_Measure_le_eq _ _ _ X_decode_le H) as [? H'];
-            rewrite H'; simpl; clear H'.
-          destruct (proj1 A_decode_pf _ _ _ _ _ (transform b1 ext0) H0 (proj1 (Ppredh _ (or_introl _ eq_refl))) Penc'') as [? [? ?]]; subst.
-          let H' := fresh in
-          destruct (Decode_w_Measure_lt_eq _ _ _ A_decode_lt H1) as [? H'];
-            rewrite H'; simpl; clear H'.
-          destruct (A_halt_dec a); simpl.
-          elimtype False; apply (proj2 (Ppredh _ (or_introl _ eq_refl)));
-            eauto.
-          eapply (fun H => IHl H _ ext0) in Penc'''; intros.
-          destruct_ex; intuition.
-          rewrite H4; simpl.
-          eexists; intuition eauto.
-          erewrite peek_correct.
-          eapply add_correct.
-          eauto.
-          eauto.
-          eauto.
-          eauto.
-      }
-      intros.
-      apply functional_extensionality; intros.
-      repeat (f_equal; repeat (apply functional_extensionality; intros)).
-      - rewrite Coq.Init.Wf.Fix_eq; simpl.
-        unfold Bind2 in Penc; computes_to_inv; injections;
-          subst; destruct v; destruct v0; destruct v1;
-            simpl in *.
-        destruct (proj1 X_decode_pf _ _ _ _ _ (transform b0 (transform b1 ext0))
-                        Eeq I Penc) as [? [? ?]]; subst.
-        rewrite <- !transform_assoc; simpl.
-        let H' := fresh in
-        destruct (Decode_w_Measure_le_eq _ _ _ X_decode_le H) as [? H'];
-          rewrite H'; simpl; clear H'.
-        destruct (proj1 A_decode_pf _ _ _ _ _ (transform b1 ext0) H0 (proj1 (Ppredh _ (or_introl _ eq_refl))) Penc') as [? [? ?]]; subst.
-        let H' := fresh in
-        destruct (Decode_w_Measure_lt_eq _ _ _ A_decode_lt H1) as [? H'];
-          rewrite H'; simpl; clear H'.
-        destruct (A_halt_dec a); simpl.
-        elimtype False; apply (proj2 (Ppredh _ (or_introl _ eq_refl)));
-          eauto.
-        eapply (fun H => IHl H _ ext0) in Penc''; intros; eauto.
-        destruct_ex; intuition.
-        rewrite H4; simpl.
-        eexists; intuition eauto.
-        erewrite peek_correct.
-        eapply add_correct.
-        eauto.
-        eauto.
-        intros.
-        apply functional_extensionality; intros.
-        repeat (f_equal; repeat (apply functional_extensionality; intros)).
     }
-    { unfold decode_list_step, encode_list_step_Spec.
+    unfold decode_DomainName, encode_DomainName_Spec; 
+      intros env env' xenv' data bin;
+      revert env env' xenv' data.
+      eapply (@well_founded_induction _ _ well_founded_lt_b) with
+      (a := bin); intros.
+      rewrite Coq.Init.Wf.Fix_eq in H2; auto using decode_body_monotone; simpl.
+
+      
+      (*{ unfold decode_list_step, encode_list_step_Spec.
       intros env env' xenv' data bin;
         revert env env' xenv' data.
       eapply (@well_founded_induction _ _ well_founded_lt_b) with
@@ -393,4 +727,5 @@ Section DomainName.
         eauto.
     }
   Qed. *)
+  Admitted.
 End DomainName.
